theories/BasicAST.v
@@ -5,3 +5,6 @@ Definition level := nat.
 Inductive mode := mKind | mType | mGhost | mProp.
 
 Inductive cmode := cType | cProp.
+
+(* Variable role: regular or parametricity. *)
+Inductive role := reg | prm.
