theories/ContextDecl.v
@@ -2,6 +2,8 @@ From Coq Require Import Utf8 List.
 From GhostTT.autosubst Require Import GAST CCAST.
 From GhostTT Require Import BasicAST.
 
+Set Primitive Projections.
+
 (** Contexts store for each variable its type and mode.
 
   The mode is redundant information already contained in the type, but we only
@@ -28,14 +30,46 @@ Notation "Γ ,, d" :=
 Notation "Γ ,,, Δ" :=
   (@app decl Δ Γ) (at level 25, Δ at next level, left associativity).
 
+(** Flex declartions for CC
 
-(** Same thing for CC **)
+  Variable handling is going to become much more complicated because erasure
+  removes some variables, while parametricity adds some in a non-uniform way
+  so computing offsets and weakenings will be painful arithmetic.
+  I propose to use flexible contexts that instead of one declaration per
+  position will have zero, one or two. A variable in the target will thus be
+  a position in the context, plus a role corresponding to how the variable is
+  used, be it as a regular or a parametricity variable.
+
+  This idea should work for all kinds of translations and is particularly suited
+  to combination of several translations like we do here.
+
+  TODO: Mention this idea of flexible variables in the paper.
+
+  We can also consider having a final translation to get rid of those but
+  this will be much nicer probably, we separate matters nicely.
+  I would argue though that we don't really need it.
+
+ **)
 
 Notation cdecl := (cmode * cterm)%type.
 
-Notation ccontext := (list cdecl).
+(* Flex declaration *)
+Record flex decl := {
+  freg : option decl ;
+  fprm : option decl
+}.
 
-Notation cscope := (list cmode).
+Arguments freg {decl}.
+Arguments fprm {decl}.
+
+Definition map_flex {d d'} (f : d → d') (c : flex d) : flex d' := {|
+  freg := option_map f c.(freg) ;
+  fprm := option_map f c.(fprm)
+|}.
+
+Notation ccontext := (list (flex cdecl)).
+
+Notation cscope := (list (flex cmode)).
 
 Definition csc (Γ : ccontext) : cscope :=
-  map fst Γ.
+  map (map_flex fst) Γ.
